examples/dm4all/IOFr2.fst
@@ -3,6 +3,8 @@ module IOFr2
 open FStar.List
 open FStar.WellFounded
 
+(* Similar to IOFr, just with uncurried WPs *)
+
 type input = int
 type output = int
 
